src/reflection/FStar.Reflection.Basic.fsti
@@ -97,7 +97,7 @@ val push_namedv    : Env.env -> bv     -> Env.env
 val range_of_term : term -> Range.range
 val range_of_sigelt : sigelt -> Range.range
 
-val subst : list subst_elt -> term -> term
+val subst_term : list subst_elt -> term -> term
 val subst_comp : list subst_elt -> comp -> comp
 
 val inspect_ident : ident -> string & Range.range
